src/Mail/MailFSStringAbsAPI.v
@@ -43,7 +43,9 @@ Module MailFSStringAbsState <: State.
   }.
 
   Definition State := state_rec.
-  Definition initP (s : State) := True.
+  Definition initP (s : State) := locked s = false /\
+                              tmpdir s = FMap.empty /\
+                              maildir s = FMap.empty.
 
 End MailFSStringAbsState.
 Module MailFSStringAbsHState := HState MailFSStringAbsState UserIdx.
